Experiments.thy
@@ -1,6 +1,7 @@
 theory Experiments
 imports Taylor_Models
 begin
+
 (*
 (* Trying out arithmetic on intervals and polynomials with interval coefficients. *)
 value "Ivl (-1::float) 1 + Ivl 0 1"
@@ -38,22 +39,24 @@ ML \<open>val test = @{code test}\<close>
 ML \<open>test ()\<close>
 ML \<open>Timing.timeit test\<close>*)
 
-value "the (compute_ivl_bound_naive 32 10 [Ivl (-1) 1] (Cos (Var 0)))"
-value "the (compute_ivl_bound_naive 32 0 [Ivl (-1) 1] (Add (Power (Cos (Var 0)) 2) (Power (Sin (Var 0)) 2)))"
-value "the (compute_ivl_bound_naive 32 10 [Ivl (-1) 1] (Add (Power (Cos (Var 0)) 2) (Power (Sin (Var 0)) 2)))"
-
 value "the (compute_tm 32 10 [Ivl (-1) 1] [0] (Cos (Var 0)))"
 value "the (compute_tm 32 10 [Ivl (-1) 1] [0] (Cos (Add (Var 0) (Mult (Num 2) Pi))))"
+value "the (compute_tm 32 10 [Ivl 9 11] [10] (Cos (Var 0)))"
+value "the (compute_tm 32 10 [Ivl (-10) 10] [0] (Cos (Var 0)))"
 value "the (compute_tm 32 10 [Ivl (-1) 1] [0] (Add (Power (Cos (Var 0)) 2) (Power (Sin (Var 0)) 2)))"
-value "the (compute_tm 64 10 [Ivl 1 3] [2] (Add (Power (Cos (Var 0)) 2) (Power (Sin (Var 0)) 2)))"
-value "the (compute_tm 32 10 [Ivl (2 - Float 1 2) (2 +  Float 1 2)] [2] (Add (Power (Cos (Add (Var 0) (Num (-2)))) 2) (Power (Sin (Add (Var 0) (Num (-2)))) 2)))"
+value "the (compute_tm 32 10 [Ivl 1 3] [2] (Add (Power (Cos (Var 0)) 2) (Power (Sin (Var 0)) 2)))"
+value "the (compute_tm 32 10 [Ivl 9 11] [10] (Add (Power (Cos (Var 0)) 2) (Power (Sin (Var 0)) 2)))"
+value "the (compute_tm 32 10 [Ivl (-1) 1] [0] (Add (Power (Cos (Add (Var 0) (Num (-2)))) 2) (Power (Sin (Add (Var 0) (Num (-2)))) 2)))"
+value "the (compute_tm 32 10 [Ivl 1 3] [2] (Add (Power (Cos (Add (Var 0) (Num (-2)))) 2) (Power (Sin (Add (Var 0) (Num (-2)))) 2)))"
 
 value "the (compute_ivl_bound 32 10 [Ivl (-1) 1] (Cos (Var 0)))"
 value "the (compute_ivl_bound 32 10 [Ivl (-1) 1] (Cos (Add (Var 0) (Mult (Num 2) Pi))))"
+value "the (compute_ivl_bound 32 10 [Ivl 9 11] (Cos (Var 0)))"
+value "the (compute_ivl_bound 32 10 [Ivl (-10) 10] (Cos (Var 0)))"
 value "the (compute_ivl_bound 32 10 [Ivl (-1) 1] (Add (Power (Cos (Var 0)) 2) (Power (Sin (Var 0)) 2)))"
-value "the (compute_ivl_bound 32 10 [Ivl 1 3]    (Add (Power (Cos (Var 0)) 2) (Power (Sin (Var 0)) 2)))"
-value "the (compute_ivl_bound 32 10 [Ivl (-1) 1] (Add (Power (Cos (Var 0)) 2) (Power (Sin (Var 0)) 2)))"
-
-find_theorems "_ (Float _ _) = (_ :: real)"
+value "the (compute_ivl_bound 32 10 [Ivl 1 3] (Add (Power (Cos (Var 0)) 2) (Power (Sin (Var 0)) 2)))"
+value "the (compute_ivl_bound 32 10 [Ivl 9 11] (Add (Power (Cos (Var 0)) 2) (Power (Sin (Var 0)) 2)))"
+value "the (compute_ivl_bound 64 5 [Ivl (Float (-1) (-4)) (Float (1) (-4))] (Add (Power (Cos (Add (Var 0) (Num (-2)))) 2) (Power (Sin (Add (Var 0) (Num (-2)))) 2)))"
+value "the (compute_ivl_bound 32 10 [Ivl 1 3] (Add (Power (Cos (Add (Var 0) (Num (-2)))) 2) (Power (Sin (Add (Var 0) (Num (-2)))) 2)))"
 
 end
